rocq-osiris/examples/proofs/inversion.v
@@ -342,7 +342,7 @@ Section verification.
       { (* Subgoal: [EWP eval_mexpr η (MStruct []) {{ ... }}]. *)
         iApply imp_module. iApply imp_sitems_extend.
         iIntros (?) "(%yl & -> & Hl)". iApply imp_sitems_nil.
-        instantiate (1 := (λ δ, ∃ yl, ⌜δ = [_]⌝ ∗ yl ↦ V #())%I).
+        instantiate (1 := (λ δ, ∃ yl, ⌜δ = [_]⌝ ∗ yl ↦ #())%I).
         by iFrame. }
       iIntros (?) "(%yl & -> & Hyl)".
 
